@prefix dc: <http://purl.org/dc/elements/1.1/> .
@prefix rdakit: <http://metadataregistry.org/uri/profile/rdakit/> .
@prefix rdf: <http://www.w3.org/1999/02/22-rdf-syntax-ns#> .
@prefix rdfs: <http://www.w3.org/2000/01/rdf-schema#> .
@prefix reg: <http://metadataregistry.org/uri/profile/RegAp/> .
@prefix skos: <http://www.w3.org/2004/02/skos/core#> .
@prefix xml: <http://www.w3.org/XML/1998/namespace> .
@prefix xsd: <http://www.w3.org/2001/XMLSchema#> .

<http://rdaregistry.info/termList/RDAproductionMethod/1003> a skos:Concept ;
    reg:identifier <http://api.metadataregistry.org/concepts/426> ;
    reg:status <http://metadataregistry.org/uri/RegStatus/1001> ;
    skos:definition "A production method consisting of a type of photolithography in which the printing plate is prepared using a bichromate process. Unhardened gelatin areas hold water and thus resist greasy ink; hardened areas accept ink and hold it in the characteristic wormlike pattern of cracks."@en ;
    skos:inScheme <http://rdaregistry.info/termList/RDAproductionMethod> ;
    skos:prefLabel "collotype"@en .

<http://rdaregistry.info/termList/RDAproductionMethod/1004> a skos:Concept ;
    reg:identifier <http://api.metadataregistry.org/concepts/427> ;
    reg:status <http://metadataregistry.org/uri/RegStatus/1001> ;
    skos:definition "A production method consisting of exposure in a camera of a silver-coated copper plate that is subsequently developed, usually using mercury vapour, and fixed with salt to create a positive image."@en ;
    skos:inScheme <http://rdaregistry.info/termList/RDAproductionMethod> ;
    skos:prefLabel "daguerreotype"@en .

<http://rdaregistry.info/termList/RDAproductionMethod/1007> a skos:Concept ;
    reg:identifier <http://api.metadataregistry.org/concepts/430> ;
    reg:status <http://metadataregistry.org/uri/RegStatus/1002> ;
    skos:inScheme <http://rdaregistry.info/termList/RDAproductionMethod> ;
    skos:prefLabel "lithograph"@en .

<http://rdaregistry.info/termList/RDAproductionMethod/1008> a skos:Concept ;
    reg:identifier <http://api.metadataregistry.org/concepts/431> ;
    reg:status <http://metadataregistry.org/uri/RegStatus/1001> ;
    skos:definition "A production method consisting of a macroform photoreproduction produced directly on opaque material by radiant energy through contact or projection."@en ;
    skos:inScheme <http://rdaregistry.info/termList/RDAproductionMethod> ;
    skos:prefLabel "photocopy"@en .

<http://rdaregistry.info/termList/RDAproductionMethod/1009> a skos:Concept ;
    reg:identifier <http://api.metadataregistry.org/concepts/432> ;
    reg:status <http://metadataregistry.org/uri/RegStatus/1001> ;
    skos:definition "A production method using a photomechanical process to prepare chemically etched printing plates."@en ;
    skos:inScheme <http://rdaregistry.info/termList/RDAproductionMethod> ;
    skos:prefLabel "photoengraving"@en .

<http://rdaregistry.info/termList/RDAproductionMethod/1010> a skos:Concept ;
    reg:identifier <http://api.metadataregistry.org/concepts/433> ;
    reg:status <http://metadataregistry.org/uri/RegStatus/1002> ;
    skos:inScheme <http://rdaregistry.info/termList/RDAproductionMethod> ;
    skos:prefLabel "print"@en .

<http://rdaregistry.info/termList/RDAproductionMethod/1011> a skos:Concept ;
    reg:identifier <http://api.metadataregistry.org/concepts/434> ;
    reg:status <http://metadataregistry.org/uri/RegStatus/1001> ;
    skos:definition "A production method consisting of copies made by light-sensitive processes, often the diazo process, usually of line drawings, in which black or coloured lines appear on a white background."@en ;
    skos:inScheme <http://rdaregistry.info/termList/RDAproductionMethod> ;
    skos:prefLabel "white print"@en .

<http://rdaregistry.info/termList/RDAproductionMethod/1012> a skos:Concept ;
    reg:identifier <http://api.metadataregistry.org/concepts/435> ;
    reg:status <http://metadataregistry.org/uri/RegStatus/1002> ;
    skos:inScheme <http://rdaregistry.info/termList/RDAproductionMethod> ;
    skos:prefLabel "woodcut"@en .

<http://rdaregistry.info/termList/RDAproductionMethod/1014> a skos:Concept ;
    reg:identifier <http://api.metadataregistry.org/concepts/1137> ;
    reg:status <http://metadataregistry.org/uri/RegStatus/1001> ;
    skos:definition "A production method consisting of an intaglio method in which the metal printing plate is prepared using a bichromate process, leaving a gelatin resist of varying thickness. The plate is etched to form cells of varying depth able to hold different amounts of ink."@en ;
    skos:inScheme <http://rdaregistry.info/termList/RDAproductionMethod> ;
    skos:prefLabel "photogravure"@en .

<http://rdaregistry.info/termList/RDAproductionMethod/1001> a skos:Concept ;
    reg:identifier <http://api.metadataregistry.org/concepts/424> ;
    reg:status <http://metadataregistry.org/uri/RegStatus/1001> ;
    skos:definition "A production method consisting of prints made on light-sensitized surfaces that produce blue images on neutral backgrounds."@en ;
    skos:inScheme <http://rdaregistry.info/termList/RDAproductionMethod> ;
    skos:prefLabel "blueline"@en ;
    skos:related <http://rdaregistry.info/termList/RDAproductionMethod/1002> .

<http://rdaregistry.info/termList/RDAproductionMethod/1002> a skos:Concept ;
    reg:identifier <http://api.metadataregistry.org/concepts/425> ;
    reg:status <http://metadataregistry.org/uri/RegStatus/1001> ;
    skos:definition "A production method consisting of a photographic process using iron salts and producing an image in Prussian blue. Blueprints are reproductive prints of architectural plans, maps, mechanical drawings, and other technical drawings, characterized by having white images on blue backgrounds."@en ;
    skos:inScheme <http://rdaregistry.info/termList/RDAproductionMethod> ;
    skos:prefLabel "blueprint"@en ;
    skos:related <http://rdaregistry.info/termList/RDAproductionMethod/1001> .

<http://rdaregistry.info/termList/RDAproductionMethod/1005> a skos:Concept ;
    reg:identifier <http://api.metadataregistry.org/concepts/428> ;
    reg:status <http://metadataregistry.org/uri/RegStatus/1001> ;
    skos:definition "A production method consisting of creating marks on the surface of a hard material, such as metal or glass, by incising with a sharp tool. In printing, the intaglio process in which the design is incised into a printing plate, usually a flat copper plate, with the aid of a graver or burin that is held in the palm of the hand and pushed against the copper to cut lines comprising V-shaped grooves. The plate is then inked up, wiped so that ink is retained in the grooves and then forced out under the pressure of the printing process to create lines on the paper. The technique was first developed in the early 15th century in Germany. Historically, \"engraving\" has sometimes been used incorrectly to refer to all printmaking processes, particularly any process employing printing plates."@en ;
    skos:inScheme <http://rdaregistry.info/termList/RDAproductionMethod> ;
    skos:prefLabel "engraving"@en ;
    skos:related <http://rdaregistry.info/termList/RDAproductionMethod/1006> .

<http://rdaregistry.info/termList/RDAproductionMethod/1006> a skos:Concept ;
    reg:identifier <http://api.metadataregistry.org/concepts/429> ;
    reg:status <http://metadataregistry.org/uri/RegStatus/1001> ;
    skos:definition "Production method consisting of an intaglio process in which the design is worked into an acid-resistant substance coating the metal printing plate; the plate is then exposed to acid, which etches the plate where the metal is exposed, to create lines and dark areas."@en ;
    skos:inScheme <http://rdaregistry.info/termList/RDAproductionMethod> ;
    skos:prefLabel "etching"@en ;
    skos:related <http://rdaregistry.info/termList/RDAproductionMethod/1005> .

<http://metadataregistry.org/uri/RegStatus/1002> a skos:Concept ;
    skos:prefLabel "New-Proposed"@en .

<http://metadataregistry.org/uri/RegStatus/1001> a skos:Concept ;
    skos:prefLabel "Published"@en .

<http://rdaregistry.info/termList/RDAproductionMethod> a skos:ConceptScheme ;
    dc:title "RDA Production Method" .

