@prefix dc: <http://purl.org/dc/elements/1.1/> .
@prefix rdakit: <http://metadataregistry.org/uri/profile/rdakit/> .
@prefix rdf: <http://www.w3.org/1999/02/22-rdf-syntax-ns#> .
@prefix rdfs: <http://www.w3.org/2000/01/rdf-schema#> .
@prefix reg: <http://metadataregistry.org/uri/profile/RegAp/> .
@prefix skos: <http://www.w3.org/2004/02/skos/core#> .
@prefix xml: <http://www.w3.org/XML/1998/namespace> .
@prefix xsd: <http://www.w3.org/2001/XMLSchema#> .

<http://rdaregistry.info/termList/rofch/T1001> a skos:Concept ;
    reg:identifier <http://api.metadataregistry.org/concepts/6918> ;
    reg:status <http://metadataregistry.org/uri/RegStatus/1001> ;
    skos:definition "Content expressed in human or machine-readable language."@en ;
    skos:inScheme <http://rdaregistry.info/termList/rofch> ;
    skos:prefLabel "language"@en .

<http://rdaregistry.info/termList/rofch/T1002> a skos:Concept ;
    reg:identifier <http://api.metadataregistry.org/concepts/6919> ;
    reg:status <http://metadataregistry.org/uri/RegStatus/1001> ;
    skos:definition "Content expressed in musical form."@en ;
    skos:inScheme <http://rdaregistry.info/termList/rofch> ;
    skos:prefLabel "music"@en .

<http://rdaregistry.info/termList/rofch/T1003> a skos:Concept ;
    reg:identifier <http://api.metadataregistry.org/concepts/6920> ;
    reg:status <http://metadataregistry.org/uri/RegStatus/1001> ;
    skos:definition "Content expressed in line, shape, mass and/or other visually-realized forms."@en ;
    skos:inScheme <http://rdaregistry.info/termList/rofch> ;
    skos:prefLabel "image"@en .

<http://rdaregistry.info/termList/rofch/T1004> a skos:Concept ;
    reg:identifier <http://api.metadataregistry.org/concepts/6921> ;
    reg:status <http://metadataregistry.org/uri/RegStatus/1001> ;
    skos:definition "Content expressed in a form other than language, music, or image."@en ;
    skos:inScheme <http://rdaregistry.info/termList/rofch> ;
    skos:prefLabel "other"@en ;
    skos:scopeNote "Includes other forms of communicating phenomena, qualities, etc., perceived directly through the human senses - e.g., natural or machine-generated sounds, aromas, textures, etc. - as well as those that cannot be perceived directly through the human senses - e.g., electromagnetic waves."@en .

<http://metadataregistry.org/uri/RegStatus/1001> a skos:Concept ;
    skos:prefLabel "Published"@en .

<http://rdaregistry.info/termList/rofch> a skos:ConceptScheme ;
    dc:title "ROF Character" .

