@prefix dc: <http://purl.org/dc/elements/1.1/> .
@prefix rdakit: <http://metadataregistry.org/uri/profile/rdakit/> .
@prefix rdf: <http://www.w3.org/1999/02/22-rdf-syntax-ns#> .
@prefix rdfs: <http://www.w3.org/2000/01/rdf-schema#> .
@prefix reg: <http://metadataregistry.org/uri/profile/RegAp/> .
@prefix skos: <http://www.w3.org/2004/02/skos/core#> .
@prefix xml: <http://www.w3.org/XML/1998/namespace> .
@prefix xsd: <http://www.w3.org/2001/XMLSchema#> .

<http://rdaregistry.info/termList/rofit/T1001> a skos:Concept ;
    reg:identifier <http://api.metadataregistry.org/concepts/6953> ;
    reg:status <http://metadataregistry.org/uri/RegStatus/1001> ;
    skos:definition "A device that magnifies microforms for reading with the unaided eye."@en ;
    skos:inScheme <http://rdaregistry.info/termList/rofit> ;
    skos:prefLabel "microform reader"@en .

<http://rdaregistry.info/termList/rofit/T1002> a skos:Concept ;
    reg:identifier <http://api.metadataregistry.org/concepts/6954> ;
    reg:status <http://metadataregistry.org/uri/RegStatus/1001> ;
    skos:definition "An instrument that magnifies objects by means of a lens or lenses so as to reveal details invisible to the naked eye."@en ;
    skos:inScheme <http://rdaregistry.info/termList/rofit> ;
    skos:prefLabel "microscope"@en .

<http://rdaregistry.info/termList/rofit/T1003> a skos:Concept ;
    reg:identifier <http://api.metadataregistry.org/concepts/6955> ;
    reg:status <http://metadataregistry.org/uri/RegStatus/1001> ;
    skos:definition "An optical device containing a light source and lens system for projecting an image on a screen or other surface."@en ;
    skos:inScheme <http://rdaregistry.info/termList/rofit> ;
    skos:prefLabel "projector"@en .

<http://rdaregistry.info/termList/rofit/T1004> a skos:Concept ;
    reg:identifier <http://api.metadataregistry.org/concepts/6956> ;
    reg:status <http://metadataregistry.org/uri/RegStatus/1001> ;
    skos:definition "An optical device with two lenses enabling each eye to see a separate image of essentially the same content to give the effect of three-dimensions."@en ;
    skos:inScheme <http://rdaregistry.info/termList/rofit> ;
    skos:prefLabel "stereoscope"@en .

<http://rdaregistry.info/termList/rofit/T1005> a skos:Concept ;
    reg:identifier <http://api.metadataregistry.org/concepts/6957> ;
    reg:status <http://metadataregistry.org/uri/RegStatus/1001> ;
    skos:definition "A device designed to play audio recordings."@en ;
    skos:inScheme <http://rdaregistry.info/termList/rofit> ;
    skos:prefLabel "audio player"@en .

<http://rdaregistry.info/termList/rofit/T1006> a skos:Concept ;
    reg:identifier <http://api.metadataregistry.org/concepts/6958> ;
    reg:status <http://metadataregistry.org/uri/RegStatus/1001> ;
    skos:definition "A device designed to play audiovisual recordings."@en ;
    skos:inScheme <http://rdaregistry.info/termList/rofit> ;
    skos:prefLabel "audiovisual player"@en .

<http://rdaregistry.info/termList/rofit/T1007> a skos:Concept ;
    reg:identifier <http://api.metadataregistry.org/concepts/6959> ;
    reg:status <http://metadataregistry.org/uri/RegStatus/1001> ;
    skos:definition "A device designed to perform prescribed sequences of operations on electronic data."@en ;
    skos:inScheme <http://rdaregistry.info/termList/rofit> ;
    skos:prefLabel "computer"@en .

<http://rdaregistry.info/termList/rofit/T1008> a skos:Concept ;
    reg:identifier <http://api.metadataregistry.org/concepts/6960> ;
    reg:status <http://metadataregistry.org/uri/RegStatus/1001> ;
    skos:definition "No intermediation tool is required (i.e., the content of the resource is directly and adequately perceivable through one or more of the human senses)."@en ;
    skos:inScheme <http://rdaregistry.info/termList/rofit> ;
    skos:prefLabel "not required"@en .

<http://metadataregistry.org/uri/RegStatus/1001> a skos:Concept ;
    skos:prefLabel "Published"@en .

<http://rdaregistry.info/termList/rofit> a skos:ConceptScheme ;
    dc:title "ROF Intermediation Tool" .

