@prefix dc: <http://purl.org/dc/elements/1.1/> .
@prefix rdakit: <http://metadataregistry.org/uri/profile/rdakit/> .
@prefix rdf: <http://www.w3.org/1999/02/22-rdf-syntax-ns#> .
@prefix rdfs: <http://www.w3.org/2000/01/rdf-schema#> .
@prefix reg: <http://metadataregistry.org/uri/profile/RegAp/> .
@prefix skos: <http://www.w3.org/2004/02/skos/core#> .
@prefix xml: <http://www.w3.org/XML/1998/namespace> .
@prefix xsd: <http://www.w3.org/2001/XMLSchema#> .

<http://rdaregistry.info/termList/rofrm/T1001> a skos:Concept ;
    reg:identifier <http://api.metadataregistry.org/concepts/6961> ;
    reg:status <http://metadataregistry.org/uri/RegStatus/1001> ;
    skos:definition "Revision through the release of notices of errors, corrections, addenda, etc."@en ;
    skos:inScheme <http://rdaregistry.info/termList/rofrm> ;
    skos:prefLabel "correction"@en .

<http://rdaregistry.info/termList/rofrm/T1002> a skos:Concept ;
    reg:identifier <http://api.metadataregistry.org/concepts/6962> ;
    reg:status <http://metadataregistry.org/uri/RegStatus/1001> ;
    skos:definition "The content is not expected to be revised after initial release."@en ;
    skos:inScheme <http://rdaregistry.info/termList/rofrm> ;
    skos:prefLabel "not applicable"@en .

<http://rdaregistry.info/termList/rofrm/T1003> a skos:Concept ;
    reg:identifier <http://api.metadataregistry.org/concepts/6963> ;
    reg:status <http://metadataregistry.org/uri/RegStatus/1001> ;
    skos:definition "Revision through the release of pages, chapters, parts, volumes, etc., directly to replace previously released counterparts, including the replacement of the entire resource with a new version."@en ;
    skos:inScheme <http://rdaregistry.info/termList/rofrm> ;
    skos:prefLabel "substitution"@en .

<http://rdaregistry.info/termList/rofrm/T1004> a skos:Concept ;
    reg:identifier <http://api.metadataregistry.org/concepts/6964> ;
    reg:status <http://metadataregistry.org/uri/RegStatus/1001> ;
    skos:definition "Revision through the incorporation of changes (including deletions) directly into the previously released content."@en ;
    skos:inScheme <http://rdaregistry.info/termList/rofrm> ;
    skos:prefLabel "transformation"@en .

<http://metadataregistry.org/uri/RegStatus/1001> a skos:Concept ;
    skos:prefLabel "Published"@en .

<http://rdaregistry.info/termList/rofrm> a skos:ConceptScheme ;
    dc:title "ROF Revision Mode" .

