@prefix rdf: <http://www.w3.org/1999/02/22-rdf-syntax-ns#> .
@prefix dc: <http://purl.org/dc/elements/1.1/> .
@prefix rdakit: <http://metadataregistry.org/uri/profile/rdakit/> .
@prefix reg: <http://metadataregistry.org/uri/profile/regap/> .
@prefix skos: <http://www.w3.org/2004/02/skos/core#> .

<http://metadataregistry.org/uri/RegStatus/1001>
    a skos:Concept ;
    skos:prefLabel "Published"@en .

<http://rdaregistry.info/termList/ModeIssue/>
    dc:title "RDA Mode of Issuance" ;
    a skos:ConceptScheme .

<http://rdaregistry.info/termList/ModeIssue/1001>
    rdakit:toolkitDefinition "A resource that is issued either as a single physical unit (e.g., as a single-volume monograph) or, in the case of an intangible resource, as a single logical unit (e.g., as a PDF file mounted on the web)."@en, "Ressource publiée comme une seule unité physique (par exemple, une monographie en un seul volume) ou, dans le cas d’une ressource immatérielle, comme une seule unité logique (par exemple, un fichier PDF installé sur le Web)."@fr, "Un recurso que fue publicado ya sea como una unidad física (por ej., una monografía de un solo volumen) o, en el caso de un recurso intangible, una sola unidad lógica (por ej., como un archivo PDF en la web)."@es, "作为独立的物理单元（例如，作为单卷本的专著），或对于一个无形的资源，作为独立的逻辑单元（例如，作为网络上登载的一个PDF文件）发行的资源。"@zh ;
    rdakit:toolkitLabel "single unit"@en, "unidad individual"@es, "unité isolée"@fr, "作为独立单元发行的资源"@zh ;
    reg:identifier <http://api.metadataregistry.org/concepts/741> ;
    reg:status <http://metadataregistry.org/uri/RegStatus/1001> ;
    a skos:Concept ;
    skos:definition "A resource that is issued either as a single physical unit (e.g., as a single-volume monograph) or, in the case of an intangible resource, as a single logical unit (e.g., as a PDF file mounted on the web)."@en, "Eine Ressource, die entweder als einzelne physische Einheit (z. B. als einbändige Monografie) oder im Falle einer immateriellen Ressource als einzelne logische Einheit erscheint (z. B. als PDF-Datei, die im Web steht)."@de, "Ressource publiée comme une seule unité physique (par exemple, une monographie en un seul volume) ou, dans le cas d’une ressource immatérielle, comme une seule unité logique (par exemple, un fichier PDF installé sur le Web)."@fr, "Un recurso que fue publicado ya sea como una unidad física (por ej., una monografía de un solo volumen) o, en el caso de un recurso intangible, una sola unidad lógica (por ej., como un archivo PDF en la web)."@es, "作为独立的物理单元（例如，作为单卷本的专著），或对于一个无形的资源，作为独立的逻辑单元（例如，作为网络上登载的一个PDF文件）发行的资源。"@zh ;
    skos:inScheme <http://rdaregistry.info/termList/ModeIssue/> ;
    skos:prefLabel "Einzelne Einheit"@de, "single unit"@en, "unidad individual"@es, "unité isolée"@fr, "作为独立单元发行的资源"@zh .

<http://rdaregistry.info/termList/ModeIssue/1002>
    rdakit:toolkitDefinition "A resource issued in two or more parts (either simultaneously or successively) that is complete or intended to be completed within a finite number of parts (e.g., a dictionary in two volumes, three audiocassettes issued as a set)."@en, "Ressource publiée en deux ou plusieurs parties (soit simultanément soit successivement) qui est complète ou destinée à l’être en un nombre déterminé de parties (par exemple, un dictionnaire en deux volumes, un jeu de trois cassettes audio)."@fr, "Un recurso editado en dos o más partes (ya sea simultáneamente o sucesivamente) que está completo o que se espera completar en un número finito de partes (por ej., un diccionario en dos volúmenes, tres audiocasetes editados como un conjunto)."@es, "以两个或两个以上的部分（同时或陆续）发行、已经出齐或计划以有限的部分出齐的资源（例如，一部两卷本的词典、作为一套发行的三盒卡式录音带）。"@zh ;
    rdakit:toolkitLabel "monografía en varias partes"@es, "monographie en plusieurs parties"@fr, "multipart monograph"@en, "多部分专著"@zh ;
    reg:identifier <http://api.metadataregistry.org/concepts/742> ;
    reg:status <http://metadataregistry.org/uri/RegStatus/1001> ;
    a skos:Concept ;
    skos:definition "A resource issued in two or more parts (either simultaneously or successively) that is complete or intended to be completed within a finite number of parts (e.g., a dictionary in two volumes, three audiocassettes issued as a set)."@en, "Eine Ressource, die (entweder gleichzeitig oder nacheinander) in mehreren Teilen erscheint, die vollständig ist oder innerhalb einer begrenzten Anzahl von Teilen abgeschlossen werden soll (z. B. ein Lexikon in zwei Bänden oder drei Audiokassetten, die als Set erscheinen)."@de, "Ressource publiée en deux ou plusieurs parties (soit simultanément soit successivement) qui est complète ou destinée à l’être en un nombre déterminé de parties (par exemple, un dictionnaire en deux volumes, un jeu de trois cassettes audio)."@fr, "Un recurso editado en dos o más partes (ya sea simultáneamente o sucesivamente) que está completo o que se espera completar en un número finito de partes (por ej., un diccionario en dos volúmenes, tres audiocasetes editados como un conjunto)."@es, "以两个或两个以上的部分（同时或陆续）发行、已经出齐或计划以有限的部分出齐的资源（例如，一部两卷本的词典、作为一套发行的三盒卡式录音带）。"@zh ;
    skos:inScheme <http://rdaregistry.info/termList/ModeIssue/> ;
    skos:prefLabel "Mehrteilige Monografie"@de, "monografía en varias partes"@es, "monographie en plusieurs parties"@fr, "multipart monograph"@en, "多部分专著"@zh .

<http://rdaregistry.info/termList/ModeIssue/1003>
    rdakit:toolkitDefinition "A resource issued in successive parts, usually bearing numbering, that has no predetermined conclusion (e.g., a periodical, a monographic series, a newspaper)."@en, "Ressource publiée en parties successives, portant en général une numérotation, sans fin prédéterminée (par exemple, un périodique, une collection de monographies, un journal)."@fr, "Un recurso publicado en partes sucesivas, generalmente con una numeración, que no tiene una conclusión determinada (por ej., una publicación periódica, una serie monográfica, un periódico)."@es, "以连续性分部方式发行的资源，通常载有编号，没有事先确定的终止期限（例如，期刊、专著丛编、报纸）。"@zh ;
    rdakit:toolkitLabel "publicación seriada"@es, "publication en série"@fr, "serial"@en, "连续出版物"@zh ;
    reg:identifier <http://api.metadataregistry.org/concepts/743> ;
    reg:status <http://metadataregistry.org/uri/RegStatus/1001> ;
    a skos:Concept ;
    skos:definition "A resource issued in successive parts, usually bearing numbering, that has no predetermined conclusion (e.g., a periodical, a monographic series, a newspaper)."@en, "Eine Ressource, die in aufeinanderfolgenden Teilen erscheint, normalerweise mit einer Zählung, die kein vorherbestimmtes Ende hat (z. B. eine Zeitschrift, eine monografische Reihe oder eine Zeitung)."@de, "Ressource publiée en parties successives, portant en général une numérotation, sans fin prédéterminée (par exemple, un périodique, une collection de monographies, un journal)."@fr, "Un recurso publicado en partes sucesivas, generalmente con una numeración, que no tiene una conclusión determinada (por ej., una publicación periódica, una serie monográfica, un periódico)."@es, "以连续性分部方式发行的资源，通常载有编号，没有事先确定的终止期限（例如，期刊、专著丛编、报纸）。"@zh ;
    skos:inScheme <http://rdaregistry.info/termList/ModeIssue/> ;
    skos:prefLabel "Fortlaufende Ressource"@de, "publicación seriada"@es, "publication en série"@fr, "serial"@en, "连续出版物"@zh ;
    skos:scopeNote "Dazu gehören Ressourcen, die Eigenschaften von fortlaufenden Ressourcen aufweisen, wie aufeinander folgende Ausgaben, Zählung und Erscheinungsfrequenz, deren Dauer jedoch begrenzt ist (z. B. Newsletter zu Ereignissen), und Reproduktionen von fortlaufenden Ressourcen."@de, "Includes resources that exhibit characteristics of serials, such as successive issues, numbering, and frequency, but whose duration is limited (e.g., newsletters of events) and reproductions of serials."@en, "Inclut les ressources présentant les caractéristiques des publications en série, telles que livraisons successives, numérotation et périodicité, mais à durée limitée (par exemple, les journaux d’événements) et les reproductions de publications en série."@fr, "Incluye recursos que presentan carácterísticas de publicaciones seriadas, tales como entregas sucesivas, numeración y frecuencia, pero cuya duración es limitada (por ej., un boletín de eventos) y reproducciones de publicaciones seriadas."@es, "包括显示连续的卷期、编号和频率等连续出版物特征，但其持续期是有限的资源（例如，事件通报）以及连续出版物的复制品。"@zh .

<http://rdaregistry.info/termList/ModeIssue/1004>
    rdakit:toolkitDefinition "A resource that is added to or changed by means of updates that do not remain discrete but are integrated into the whole (e.g., a loose-leaf manual that is updated by means of replacement pages, a website that is updated continuously)."@en, "Ressource augmentée ou modifiée par des mises à jour qui ne restent pas distinctes, mais qui sont intégrées à l’ensemble de la ressource. Une ressource intégratrice peut être matérielle (par exemple, un manuel à feuillets mobiles mis à jour par de nouvelles pages) ou immatérielle (par exemple, un site Web mis à jour soit de façon permanente soit de façon périodique."@fr, "Un recurso que es añadido o cambiado por medio de actualizaciones que no estan separadas sino integradas en el todo (por ej., un manual de hojas sueltas que se actualiza mediante hojas intercambiables, un sitio web que se actualiza continuamente)."@es, "以更新的方式进行增补或更改的资源，更新部分与整体不是分离的而是融为一体的。集成性资源可以是有形的（例如，通过换页方式进行更新的活页手册）或无形的（例如，通过持续或循环的方式进行更新的网站）。"@zh ;
    rdakit:toolkitLabel "integrating resource"@en, "recurso integrable"@es, "ressource intégratrice"@fr, "集成性资源"@zh ;
    reg:identifier <http://api.metadataregistry.org/concepts/744> ;
    reg:status <http://metadataregistry.org/uri/RegStatus/1001> ;
    a skos:Concept ;
    skos:definition "A resource that is added to or changed by means of updates that do not remain discrete but are integrated into the whole (e.g., a loose-leaf manual that is updated by means of replacement pages, a website that is updated continuously)."@en, "Eine Ressource, die durch Aktualisierungen ergänzt oder verändert wird, die nicht getrennt bleiben, sondern in das Ganze integriert werden (z. B. ein Handbuch in Loseblattform, das durch Austausch von Seiten aktualisiert wird, eine Web-Site, die entweder kontinuierlich oder in regelmäßigen Abständen aktualisiert wird)."@de, "Ressource augmentée ou modifiée par des mises à jour qui ne restent pas distinctes, mais qui sont intégrées à l’ensemble de la ressource. Une ressource intégratrice peut être matérielle (par exemple, un manuel à feuillets mobiles mis à jour par de nouvelles pages) ou immatérielle (par exemple, un site Web mis à jour soit de façon permanente soit de façon périodique."@fr, "Un recurso que es añadido o cambiado por medio de actualizaciones que no estan separadas sino integradas en el todo (por ej., un manual de hojas sueltas que se actualiza mediante hojas intercambiables, un sitio web que se actualiza continuamente)."@es, "以更新的方式进行增补或更改的资源，更新部分与整体不是分离的而是融为一体的。集成性资源可以是有形的（例如，通过换页方式进行更新的活页手册）或无形的（例如，通过持续或循环的方式进行更新的网站）。"@zh ;
    skos:inScheme <http://rdaregistry.info/termList/ModeIssue/> ;
    skos:prefLabel "Integrierende Ressource"@de, "integrating resource"@en, "recurso integrable"@es, "ressource intégratrice"@fr, "集成性资源"@zh .

